
\documentclass{article}

\usepackage{amsmath}
\usepackage{amsfonts}
\usepackage{amssymb}
\usepackage{enumerate}
\usepackage{mathtools}
\usepackage{xfrac}
\usepackage[lastexercise]{exercise}

\DeclarePairedDelimiter\floor{\lfloor}{\rfloor}

\newcounter{Problem}
\newenvironment{Problem}{\begin{Exercise}[name={Problem},
                                          counter={Problem}]}
                        {\end{Exercise}}
\title{MATH 829 Homework \#4}
\date{February 11, 2015}
\author{Sam Boling}

\begin{document}

\begin{titlepage}
\maketitle
\end{titlepage}

\section{Textbook Problems}

\subsection*{Ch. II \S 5.1}
Define
$$
a_k
=
\left\{\begin{array}{l l}
  \frac{1}{k!}, & \quad k \text{ even} \\
  0,            & \quad k \text{ odd}
\end{array}\right.
$$
so that
$$
f(z) = \sum_{n=0}^{\infty} \frac{z^{2n}}{(2n)!} = \sum_{k=0}^\infty a_k z^k.
$$
Then
\begin{align*}
   f^{\prime\prime}(z)
&= \sum_{k=2}^\infty k (k-1) a_k z^{k-2}
&= \sum_{k \in 2\mathbb{N}} \frac{z^{k-2}}{(k-2)!} \\
&= \sum_{n \in \mathbb{N}} \frac{z^{2n - 2}}{(2n - 2)!}
\end{align*}
under the substitution $k = 2n$, so that
\begin{align*}
   f^{\prime\prime}(z)
&= \sum_{n=1}^\infty \frac{z^{2n - 2}}{(2n - 2)!}
 = \sum_{n=1}^\infty \frac{z^{2(n-1)}}{(2(n-1))!} \\
&= \sum_{n=0}^\infty \frac{z^{2n}}{(2n)!}
 = f(z).
\end{align*}

We observe also that under the substitution $w = z^2$ this is
the series
$$
\sum_{n=0}^{\infty} \frac{w^n}{(2n)!}
$$
which has radius of convergence $\infty$ since
$$
\lim \frac{|(2n)!|}{|(2n+1)!} = \frac{1}{2n+1} = 0
$$
and so $f(z)$ has radius of convergence $\infty$ as well.

\subsection*{Ch. II \S 5.4}
Let $w = \left(\frac{z}{2}\right)^2$ so that
$\frac{dw}{dz} = \frac{z}{2}$
and $\frac{d^2w}{dz^2} = \frac{1}{2}$.
Then
$$
J(z) = \sum_{n=0}^\infty \frac{(-1)^n}{(n!)^2} w^n
$$
so that
\begin{align*}
   \frac{dJ}{dz}
&= \frac{dJ}{dw}\frac{dw}{dz}
 = \frac{z}{2}\sum_{n=1}^\infty \frac{n (-1)^n}{(n!)^2} w^{n-1} \\
&= \frac{z}{2}
   \sum_{n=1}^\infty
     \frac{n (-1)^n}{(n!)^2}
     \left(\frac{z}{2}\right)^{2(n-1)}
\end{align*}
and
\begin{align*}
   \frac{d^2J}{dz^2}
&= \frac{d^2J}{dw^2}\left(\frac{dw}{dz}\right)^2
 + \frac{dJ}{dw}\frac{d^2w}{dz^2} \\
&= \left(\frac{z}{2}\right)^2
   \sum_{n=2}^\infty
     n (n-1)
     \frac{(-1)^n}{(n!)^2}
     w^{n-2}
  + \frac{1}{2}
    \sum_{n=1}^\infty
      n \frac{(-1)^n}{(n!)^2} w^{n-1} \\
&= \sum_{n=2}^\infty
     n (n-1)
     \frac{(-1)^n}{(n!)^2}
     w^{n-1}
  + \frac{1}{2}
    \sum_{n=1}^\infty
      n \frac{(-1)^n}{(n!)^2} w^{n-1} \\
&= -\frac{1}{2}
 +  \sum_{n=2}^\infty
      n \frac{(-1)^n}{(n!)^2}
      (n - 1 + 1) w^{n-1} \\
&= -\frac{1}{2}
 + \sum_{n=2}^\infty
   \frac{(-1)^n}{((n-1)!)^2} w^{n-1} \\
&= -\frac{1}{2}
 + \sum_{n=1}^\infty
     \frac{(-1)^{n+1}}{(n!)^2}
     \left(\frac{z}{2}\right)^{2n}
\end{align*}

%Letting $w = z^2$, we write
%$$
%  \sum_{n=0}^\infty \frac{(-1)^n}{(n!)^2 2^{2n}} z^{2n}
%= \sum_{n=0}^\infty \frac{(-1)^n}{(n!)^2 2^{2n}} w^n
%$$
%and compute
%\begin{align*}
%   \frac{dJ}{dw}
%&= \sum_{n=1}^\infty
%     n
%     \frac{(-1)^n}{(n!)^2 2^{2n}} w^{n-1}
%\end{align*}
%so that
%\begin{align*}
%   \frac{dJ}{dz}
%&= \frac{dw}{dz}\frac{dJ}{dw}
% = 2z
%   \sum_{n=1}^\infty
%     n
%     \frac{(-1)^n}{(n!)^2 2^{2n}} z^{2(n-1)} \\
%&= \sum_{n=1}^\infty
%     n
%     \frac{(-1)^n}{(n!)^2 2^{2n-1}} z^{2n-1}.
%\end{align*}
%Furthermore we find that
%\begin{align*}
%   \frac{d^2 J}{dw^2}
%&= \sum_{n=2}^\infty
%     n (n-1)
%     \frac{(-1)^n}{(n!)^2 2^{2n}}
%     w^{n-2}
% = \sum_{n=2}^\infty
%     n (n-1)
%     \frac{(-1)^n}{(n!)^2 2^{2n}}
%     z^{2(n-2)}
%\end{align*}
%so that
%\begin{align*}
%   \frac{d^2 J}{dz^2}
%&= \frac{d^2 J}{dw^2} \left(\frac{dw}{dz}\right)^2
% + \frac{dJ}{dw} \frac{d^2w}{dz^2} \\
%&= (2z)^2 \frac{d^2J}{dw^2} + 2 \frac{dJ}{dw} \\
%&= \sum_{n=2}^\infty
%     n (n-1)
%     \frac{(-1)^n}{(n!)^2 2^{2n-2}}
%     z^{2n-2}
% + 2\sum_{n=1}^\infty
%      n
%      \frac{(-1)^n}{(n!)^2 2^{2n}}
%      z^{2(n-1)} \\
%&= \sum_{n=2}^\infty
%     n (n-1)
%     \frac{(-1)^n}{(n!)^2 2^{2(n-1)}}
%     z^{2(n-1)}
% + \frac{1}{2}
%   \sum_{n=1}^\infty
%     n
%     \frac{(-1)^n}{(n!)^2 2^{2(n-1)}}
%     z^{2(n-1)} \\
%&= -\frac{1}{2}
% + \sum_{n=2}^\infty
%     ((n-1) + 1)
%     n
%     \frac{(-1)^n}{(n!)^2 2^{2(n-1)}}
%     z^{2(n-1)} \\
%&= -\frac{1}{2}
% + \sum_{n=2}^\infty
%     \frac{(-1)^n}{((n-1)!)^2 2^{2(n-1)}}
%     z^{2(n-1)} \\
%&= -\frac{1}{2}
% + \sum_{n=1}^\infty
%     \frac{(-1)^{n+1}}{(n!)^2 2^{2n}}
%     z^{2n}.
%\end{align*}
%This means that
%\begin{align*}
%   z^2 J(z) + z^2 J^{\prime\prime}(z)
%&= z^2
%   \sum_{n=0}^\infty
%     \frac{(-1)^n}{(n!)^2 2^{2n}}
%     z^{2n}
% - \frac{z^2}{2}
% + z^2
%   \sum_{n=1}^\infty
%     \frac{(-1)^{n+1}}{(n!)^2 2^{2n}}
%     z^{2n} \\
%&= \frac{z^2}{2}
%\end{align*}

%hen notice
%begin{align*}
%  J^\prime(z)
%= \sum_{n=1}^\infty
%    n
%    \frac{(-1)^n}{(n!)^2 2^{2n-1}}
%    z^{2n-1} \\
%= \frac{z}{2}
%  \sum_{n=1}^\infty
%    \frac{(-1)^n}{n! (n-1)! 2^{2(n-1)}} z^{2(n-1)} \\
%= \frac{z}{2}
%  \sum_{n=0}^\infty
%     \frac{(-1)^{n+1}}{n! (n+1)!}
%     \left(\frac{z}{2}\right)^{2n} \\
%= \sum_{n=0}^\infty
%     \frac{(-1)^{n+1}}{n! (n+1)!}
%     \left(\frac{z}{2}\right)^{2n+1}
%end{align*}
%nd
%begin{align*}
%  J^{\prime\prime}(z)
%= \sum_{n=2}^\infty
%    n(n-1)
%    \frac{(-1)^n}{(n!)^2 2^{2(n-1)}} z^{2(n-1)}
%+ 2\sum_{n=1}^\infty
%  \\
%= \sum_{n=1}^\infty
%    n(n+1)
%    \frac{(-1)^{n+1}}{((n+1)!)^2}
%    \left(\frac{z}{2}\right)^{2n}
%+ 2\sum_{n=1}^\infty \\
%end{align*}
%o that
%begin{align*}
%& z^2 J^{\prime\prime}(z) + z J^\prime(z) + z^2 J(z) \\
%&
%end{align*}

%\begin{align*}
% &  z^2 J^{\prime\prime}(z) + z J^\prime(z) + z^2 J(z) \\
%=& \sum_{n=2}^\infty
%     n(n-1)
%     \frac{(-1)^n}{(n!)^2 2^{2(n-1)}}
%     z^{2n}
%+ \sum_{n=1}^\infty
%     n
%     \frac{(-1)^n}{(n!)^2 2^{2n}}
%     z^{2(n+1)} \\
%+& \sum_{n=1}^\infty
%     n
%     \frac{(-1)^n}{(n!)^2 2^{2n-1}}
%     z^{2n} \\
%+& \sum_{n=0}^\infty
%     \frac{(-1)^n}{(n!)^2 2^{2n}}
%     z^{2(n+1)} \\
%=& \sum_{n=2}^\infty
%     n(n-1)
%     \frac{(-1)^n}{(n!)^2 2^{2(n-1)}}
%     z^{2n}
%+ \left(-\frac{1}{4} z^4\right)
%+ \sum_{n=2}^\infty
%    n
%    \frac{(-1)^n}{(n!)^2 2^{2n}}
%    z^{2(n+1)} \\
%+& \left(-\frac{1}{2} z^2\right)
%+ \sum_{n=2}^\infty
%    n
%    \frac{(-1)^n}{(n!)^2 2^{2n-1}}
%    z^{2n} \\
%+& z^2
%- \frac{1}{4} z^4
%+ \sum_{n=2}^\infty
%    \frac{(-1)^n}{(n!)^2 2^{2n}}
%    z^{2(n+1)} \\
%=& \frac{1}{2} z^2
%-  \frac{1}{2} z^4
%+  \sum_{n=2}^\infty
%     n(n-1)
%\end{align*}

%Then rearranging,
%\begin{align*}
%   J^{\prime}(z)
%&= 2z \sum_{n=1}^\infty n \frac{(-1)^n}{(n!)^2 2^{2n}} z^{2n-2} \\
%&= 2z \sum_{n=0}^\infty (n+1) \frac{(-1)^{n+1}}{((n+1)!)^2 2^{2(n+1)}}
%  (z^2)^n
%\end{align*}
%so that
%$$
%  z J^\prime(z)
%= 2w
%  \sum_{n=0}^\infty
%    (n+1)
%    \frac{(-1)^{n+1}}{((n+1)!)^2 2^{2(n+1)}}
%    w^n
%$$
%and so
%\begin{align*}
%   J^{\prime\prime}(z)
%&= \frac{d}{dz}\left(\frac{dJ}{dz}\right)
% = \frac{d}{dz}\left(\frac{dJ}{dw}\frac{dw}{dz}\right) \\
%&= \frac{d}{dz}\left(2z J^\prime(w(z))\right)
% = 2 J^\prime(w) + 2z \frac{dw}{dz} \frac{dJ^\prime}{dw} \\
%&= 2 \sum_{n=1}^\infty
%     n
%     \frac{(-1)^n}{(n!)^2 2^{2n}} w^{n-1}
% + (2z)^3
%   \sum_{n=1}^\infty
%     n (n+1) \frac{(-1)^{n+1}}{((n+1)!)^2 2^{2(n+1)}} w^{n-1} \\
%&= 2 \sum_{n=1}^\infty
%     n
%     \frac{(-1)^n}{(n!)^2 2^{2n}} z^{2(n-1)}
% + (2z)^3
%   \sum_{n=1}^\infty
%     n (n+1) \frac{(-1)^{n+1}}{((n+1)!)^2 2^{2(n+1)}} z^{2(n-1)} \\
%&= 2 \sum_{n=1}^\infty
%     n
%     \frac{(-1)^n}{(n!)^2 2^{2n}} z^{2(n-1)}
% + 2z
%   \sum_{n=1}^\infty
%     n (n+1) \frac{(-1)^{n+1}}{((n+1)!)^2 2^{2n}} z^{2n} \\
%&= 2 \sum_{n=1}^\infty
%     n
%     \frac{(-1)^n}{(n!)^2 2^{2n}} z^{2(n-1)}
% + 2z
%   \sum_{n=1}^\infty
%     \frac{1}{n+1}
%     n
%     \frac{(-1)^{n+1}}{(n!)^2 2^{2n}} z^{2n} \\
%&= 2 \sum_{n=1}^\infty
%     n
%     \frac{(-1)^n}{(n!)^2 2^{2n}}
%     \left[z^{2(n-1)} - \frac{z^{2n+1}}{n+1}\right]
%\end{align*}
%
%so that
%\begin{align*}
%   z^2 J^{\prime\prime}(z) + z J^\prime(z) + z^2 J(z)
%&= 2\sum_{n=1}^\infty
%      n
%      \frac{(-1)^n}{(n!)^2 2^{2n}}
%      z^{2n} \\
%&+ (2z)^3 \sum_{n=1}^\infty
%      n (n+1)
%      \frac{(-1)^{n+1}}{((n+1)!)^2 2^{2(n+1)}} z^{2n} \\
%&+ \sum_{n=1}^\infty
%     n
%     \frac{(-1)^n}{(n!)^2 2^{2n-1}} z^{2n}
%&+ \sum_{n=0}^\infty
%     \frac{(-1)^n}{(n!)^2 2^{2n}} z^{2(n+1)}
%\end{align*}

% Defining
%$$
%a_k
%=
%\left\{\begin{array}{l l}
%  \frac{(-1)^{\frac{k}{2}}}{\left(\frac{k}{2}!\right)^2 2^k},
%    & \quad k \text{ even} \\
%  0 & \quad k \text{ odd}
%\end{array}\right.,
%$$
%we can write
%$$
%  J(z)
%= \sum_{n=0}^\infty \frac{(-1)^n}{(n!)^2}\left(\frac{z}{2}\right)^{2n}
%= \sum_{k=0}^\infty a_k z^k
%$$
%so that
%\begin{align*}
%   J^\prime(z)
%&= \frac{d}{dz} \sum_{k=0}^\infty a_k z^k
% = \sum_{k=1}^\infty k a_k z^{k-1} \\
%&= \sum_{k=2}^\infty k a_k z^{k-1}
% = \sum_{k \in 2\mathbb{N}} k a_k z^{k-1} \\
%&= \sum_{k \in 2\mathbb{N}} k \frac{(-1)^{\frac{k}{2}}}{\left(\frac{k}{2}!\right)^2 2^k} z^{k-1}
%\end{align*}
%since $a_1 = 0$. But then by substituting $n = 2k$,
%\begin{align*}
%   J^\prime(z)
%&= \sum_{n=1}^\infty 2n \frac{(-1)^{n}}{(n!)^2 2^{2n}} z^{2n-1}
% = \sum_{n=1}^\infty \frac{(-1)^n}{(n-1)! \cdot n! \cdot 2^{2n-1}} z^{2n-1}.
%\end{align*}
%By the same procedure
%\begin{align*}
%   J^{\prime\prime}(z)
%&= \sum_{k=2}^\infty k (k-1) a_k z^{k-2}
% = \sum_{n=1}^\infty 2n (2n-1) \frac{(-1)^{n}}{(n!)^2 2^{2n}} z^{2n-2} \\
%&= \sum_{n=1}^\infty (2n-1) \frac{(-1)^n}{(n-1)! \cdot n! \cdot 2^{2n-1}} z^{2n-2}.
%\end{align*}
%Then
%\begin{align*}
%   z^2 J^{\prime\prime}(z) + z J^\prime(z) + z^2 J(z)
%&= \sum_{n=1}^\infty (2n-1) \frac{(-1)^n}{(n-1)! \cdot n! \cdot 2^{2n-1}} z^{2n} \\
%&+ \sum_{n=1}^\infty \frac{(-1)^n}{(n-1)! \cdot n! \cdot 2^{2n-1}} z^{2n} \\
%&+ \sum_{n=0}^\infty \frac{(-1)^n}{(n!)^2 2^{2n}} z^{2n + 2} \\
%&= z^2 + \sum_{n=1}^\infty
%\end{align*}

\subsection*{Ch. II \S 5.6(a)}
Observe that by a change of index $k = n+1$
\begin{align*}
   \log z
&= \sum_{n=1}^\infty \frac{(-1)^{n-1}}{n}(z-1)^n
 = \sum_{n=0}^\infty \frac{(-1)^n}{n+1} (z-1)^{n+1} \\
&= (z-1)\sum_{n=0}^\infty \frac{(-1)^n}{n+1}
\end{align*}
so that
\begin{align*}
   \frac{d}{dz} \log z
&= \left[\frac{d}{dz} (z-1)\right]
   \sum_{n=0}^\infty \frac{(-1)^n}{n+1} (z-1)^n
 + (z-1)\sum_{n=1}^\infty n\frac{(-1)^n}{n+1} (z - 1)^{n-1} \\
&= \sum_{n=0}^\infty \frac{(-1)^n}{n+1} (z-1)^n
 + \sum_{n=1}^\infty n \frac{(-1)^n}{n+1} (z-1)^n \\
&= 1 + \sum_{n=1}^\infty (1 + n) \frac{(-1)^n}{n+1} (z-1)^n \\
&= 1 + \sum_{n=1}^\infty (-1)^n (z-1)^n \\
&= \sum_{n=0}^\infty (1-z)^n,
\end{align*}
and when $|z - 1| < 1$ this geometric series converges to
$$
\frac{d}{dz} \log z = \frac{1}{1 - (1 - z)} = \frac{1}{z}.
$$

\section{Additional Problems}

\begin{Problem}
  Prove that $\sum_{n=0}^\infty z^n$ does not converge uniformly on
  $D(0, 1)$.
\end{Problem}

\begin{Answer}
  We consider the sequence $(f_n)$ given by
  $$
  f_n(z) = \sum_{k=0}^n z^k,
  $$
  since by definition $\sum_{n=0}^\infty z^n$ is the limit
  of this sequence.

  For any $n$, we can compute the supremum norm
  \begin{align*}
    \left\|
      f_{n+1} - f_n
    \right\|_{D(0,1)}
  &=
    \left\|
      \sum_{k=0}^{n+1} z^k
    - \sum_{k=0}^{n} z^k
    \right\|_{D(0,1)}
   =
  \left\|
    z^{n+1}
  \right\|_{D(0,1)} \\
  &=
  \sup_{D(0,1)} |z^{n+1}|
   =
  \sup_{D(0,1)} |z|^{n+1}
   = 1
  \end{align*}
  and therefore the sequence $(f_n)$ is not uniformly
  Cauchy.
\end{Answer}

\begin{Problem}
  Let $f$ be analytic on an open set $U$. Let
  $V = \{ z \in \mathbb{C} : \bar{z} \in U \}$. Define $g$ on $V$ by
  $g(z) = \overline{f(\bar{z})}$. Show that $g$ is analytic on $V$.
\end{Problem}

\begin{Answer}
For $z_0 \in V$ we have $\bar{z_0} \in U$, so
$f$ is analytic at $\bar{z_0}$, so there is an
$r > 0$ and a sequence $(a_n)$ such that
$$
  f(w)
= \sum_{n=0}^\infty a_n(w - \bar{z_0})^n, \quad
  |w - z_0| < r.
$$

Now let $z \in D(z_0, r)$, and write $z = a + ib$ and
$z_0 = a_0 + ib_0$. Then $|z - z_0| < r$, but we note that
\begin{align*}
  |z - z_0|
&= |(a + ib) - (a_0 + ib_0)|
 = |(a - a_0) + i(b - b_0)| \\
&= \sqrt{(a - a_0)^2 + (b - b_0)^2}
\end{align*}
while
\begin{align*}
  |\bar{z} - \bar{z_0}|
&= |(a - ib) - (a_0 - ib_0)|
 = |(a - a_0) + i(-b + b_0)| \\
&= \sqrt{(a - a_0)^2 + (b_0 - b)^2}
 = \sqrt{(a - a_0)^2 + (b - b_0)^2} \\
&= |z - z_0|,
\end{align*}
so if $z \in D(z_0, r)$ then $\bar{z} \in D(\bar{z_0}, r)$. Therefore
the expression
$$
f(\bar{z})
= \sum_{n=0}^\infty a_n (\bar{z} - \bar{z_0})^n
$$
holds, so
$$
  g(z)
= \overline{f(\bar{z})}
= \sum_{n=0}^\infty \frac{\overline{f^{(n)}(\bar{z_0})}}{n!}
                 \overline{(\bar{z} - \bar{z_0})^n}
= \sum_{n=0}^\infty \frac{\overline{f^{(n)}(\bar{z_0})}}{n!}
                 (z - z_0)^n, \quad
|z - z_0| < r.
$$
Since $z_0$ was chosen arbitrarily
in $V$, this means $g$ is analytic on $V$.
\end{Answer}

\begin{Problem}
  Let $U$ be a domain such that $\forall z \in U$, $\bar{z} \in U$.
  \begin{enumerate}[(i)]
    \item{
      Show that $U \cap \mathbb{R}$ contains an open interval.
    }
    \item{
      Let $f$ be analytic on $U$. Suppose that $f(x) \in \mathbb{R}$
      $\forall x \in U \cap \mathbb{R}$. Show that $f(\bar{z}) = \overline{f(z)}$
      for all $z \in U$.
    }
  \end{enumerate}
\end{Problem}

\begin{Answer}
  \begin{enumerate}
    \item{
      Since $U$ is nonempty, let $z_0 \in U$.

      If $\mathrm{Im}~z_0 = 0$
      then $z_0 \in \mathbb{R}$, and since $U$ is open there is a disk
      $D(z_0, r) \subset U$ for some $r > 0$. Then
      $$
        D(z_0, r) \cap \mathbb{R}
      = \{ z \in \mathbb{R} : |z - z_0| < r \}
      = (z-r, z+r),
      $$
      an open interval in
      $\mathbb{R} \cap D(z_0, r) \subset \mathbb{R} \cap U$.

      Suppose $\mathrm{Im}~z_0 \neq 0$. Without loss of generality,
      let $\mathrm{Im}~z_0 > 0$ so that $z_0$ lies in the upper half-plane
      $\{ z \in \mathbb{C} : \mathrm{Im}~z > 0 \}$. Then
      by assumption $\bar{z_0} \in U$, and
      $\mathrm{Im}~\bar{z_0} = -\mathrm{Im}~\bar{z_0}$ so
      $\bar{z_0} \in \{ z \in \mathbb{C} : \mathrm{Im}~z < 0 \}$.
      Then since $U$ is open and connected it is path-connected, so
      there exists a continuous function $\gamma: [0, 1] \to U$ such
      that $\gamma(0) = z_0$ and $\gamma(1) = \bar{z_0}$. But
      $\mathrm{Im}$ is continuous and thus so is
      $\mathrm{Im} \circ \gamma$, so from the intermediate value
      theorem there must be some $x \in [0, 1]$ such that
      $\Im(\gamma(x)) = 0$. Then since $\gamma(x) \in U$, the case
      where $\mathrm{Im}~z_0 = 0$ can be applied to find an open
      interval $(\gamma(x) - r, \gamma(x) + r)$ for some $r > 0$.
    }
    \item{
      Under our assumption the set
      $$
      V = \{ z \in \mathbb{C} : \bar{z} \in U \}
      $$
      is equal to $U$, and in the previous problem we saw that
      this means $g(z) = \overline{f(\bar{z})}$ is analytic on
      $U$.

      Let $x \in U \cap \mathbb{R}$. Then
      $x = \bar{x}$ and by assumption $f(x) \in \mathbb{R}$,
      so $g(x) = \overline{f(\bar{x})} = f(x)$ on $U \cap \mathbb{R}$.
      But we saw that $U \cap \mathbb{R}$ contains an open
      interval $(x_0 - r, x_0 + r)$ for some $x_0 \in \mathbb{R}$,
      $r > 0$, and certainly either of these endpoints is an
      accumulation point of $U \cap \mathbb{R}$ since
      the sequence $x_0 - r + \frac{1}{n} \to x_0 - r$.
      From the uniqueness theorem for analytic functions this means
      that $f(z) = g(z)$ in $U$, i.e. $f(z) = \overline{f(\bar{z})}$ so
      $\overline{f(z)} = f(\bar{z})$ on $U$ as desired.
    }
  \end{enumerate}
\end{Answer}

\begin{Problem}
  Show that there does not exist a function which is analytic on
  $\mathbb{C}$ that satisfies
  $f\left(\frac{1}{n}\right) = \left|\frac{1}{n^3}\right|$ for all
  $n \in \mathbb{Z} \backslash \{ 0 \}$.
\end{Problem}

\begin{Answer}
  The function $g(z) = z^3$ is a polynomial and therefore analytic
  on $\mathbb{C}$. But $g(z) = f(z)$ for any $z = \frac{1}{n}$ where
  $n \in \mathbb{N} \subset \mathbb{Z} \backslash \{0\},$, and the set
  $$
  \left\{\frac{1}{n} : n \in \mathbb{N} \right\}
  $$
  has an accumulation point at $0 \in \mathbb{C}$. From the uniqueness theorem
  this means that $f = g$ in $\mathbb{C}$, which is a contradiction
  since $f(-1) = -1 \neq 1 = g(-1)$ by definition.
\end{Answer}

\end{document}
