
\documentclass{article}

\usepackage{amsmath}
\usepackage{amsfonts}
\usepackage{amssymb}
\usepackage{enumerate}
\usepackage{mathtools}
\usepackage{xfrac}
\usepackage[lastexercise]{exercise}

\DeclarePairedDelimiter\floor{\lfloor}{\rfloor}

\newcounter{Problem}
\newenvironment{Problem}{\begin{Exercise}[name={Problem},
                                          counter={Problem}]}
                        {\end{Exercise}}
\title{MATH 829 Homework \#3}
\date{February 4, 2015}
\author{Sam Boling}

\begin{document}

\begin{titlepage}
\maketitle
% TODO: III.6.2?
\end{titlepage}

\section{Textbook Problems}

\subsection*{Ch. II, \S 2.4}
\begin{itemize}
  \item[(a)]{
    The series
    $$
    \sum_{n=0}^\infty n^n z^n
    $$
    has $a_n = n^n$ so that
    $$
      \limsup |a_n|^{1 / n}
    = \limsup (n^n)^{1 / n}
    = \limsup n = \infty,
    $$
    and therefore $R = 0$.
  }
  \item[(c)]{
    The series
    $$
    \sum_{n=0}^\infty 2^n z^n
    $$
    has
    $$
      \left|\frac{a_{n+1}}{a_n}\right|
    = \frac{2^{n+1}}{2^n}
    = 2
    $$
    so that $R = \frac{1}{2}$.
  }
  \item[(f)]{
    The series
    $$
    \sum_{n=0}^\infty n^2 z^n
    $$
    has
    $$
      \left|\frac{a_{n+1}}{a_n}\right|
    = \frac{n^2 + 2n + 1}{n^2}
    = 1 + 2\frac{1}{n} + \frac{1}{n^2} \to 1
    $$
    so that $R = 1$.
  }
  \item[(g)]{
    The series
    $$
    \sum_{n=0}^\infty \frac{n!}{n^n} z^n
    $$
    has
    \begin{align*}
      \frac{|a_{n+1}|}{|a_n|}
    &= \frac{\frac{(n+1)!}{(n+1)^{n+1}}}
            {\frac{n!}{n^n}}
     = n\frac{n^n}{(n+1)^{n+1}}
     = \frac{n}{n+1} \left(\frac{n}{n+1}\right)^n \\
    &= \left(\frac{n}{n+1}\right)^{n+1}
     = \left(1 + \frac{1}{n}\right)^{-(n+1)}
     = \frac{1}{\left(1 + \frac{1}{n}\right)^{n+1}} \\
    &= \frac{1}{\left(1 + \frac{1}{n}\right)^n}
       \frac{1}{\left(1 + \frac{1}{n}\right)}
     \to \frac{1}{e},
    \end{align*}
    so $R = e$.
  }
\end{itemize}

\subsection*{Ch. II \S 2.10}
\begin{enumerate}[(a)]
  \item{
    Noting that
    $\sum (a_n + b_n) z^n = \sum a_n z^n + \sum b_n z^n$
    so that
    $$
      \lim_{n \to \infty} \sum_{k=0}^n (a_k + b_k) z^k
    = \lim_{n \to \infty} \sum_{k=0}^n a_k z^k
    + \lim_{n \to \infty} \sum_{k=0}^n b_k z^k,
    $$
    we see that this series is convergent only if
    both $\sum a_n z^n$ and $\sum b_n z^n$ converge. Therefore
    the region of convergence is the intersection of the
    regions of convergence of these two series, i.e.
    $D(0, r) \cap D(0, s)$, so the region of convergence is
    given by $\min(r, s)$.
  }
  \item{
    We see that
    \begin{align*}
       \lim_{n \to \infty} \left|\frac{a_{n+1} b_{n+1}}{a_n b_n}\right|
    &= \lim_{n \to \infty} \left|\frac{a_{n+1}}{a_n}\right|
                       \left|\frac{b_{n+1}}{b_n}\right|
     = \left(\lim_{n \to \infty}
        \left|\frac{a_{n+1}}{a_n}\right|
       \right)
       \left(\lim_{n \to \infty}
         \left|\frac{b_{n+1}}{b_n}\right|
       \right) \\
    &= \frac{1}{r} \frac{1}{s}
     = \frac{1}{rs}
    \end{align*}
    so that the radius of convergence is $rs$.
  }
\end{enumerate}

\subsection*{Ch. III \S 6.1}
\begin{itemize}
  \item[(d)]{
    $i^i = e^{i \log i}$,
    and $i = e^{i \frac{\pi}{2}}$ so for this branch of the logarithm
    we have $\log i = i\frac{\pi}{2}$. Then
    $e^{i \log i} = e^{-\frac{\pi}{2}}$.
  }
  \item[(e)]{
    $(-i)^i = e^{i \log (-i)}$, and $-i = e^{-i\frac{\pi}{2}}$ so for
    this branch of the logarithm we have $\log i = -i\frac{\pi}{2}$,
    so $(-i)^i = e^{\frac{\pi}{2}}$.
  }
\end{itemize}

\subsection*{Ch. III \S 6.2}
\begin{itemize}
  \item[(d)]{
    $i^i = e^{i \log i}$,
    and $i = e^{i \frac{\pi}{2}}$ so for this branch of the logarithm
    we have $\log i = i\frac{\pi}{2}$. Then
    $e^{i \log i} = e^{-\frac{\pi}{2}}$. The same value is attained
    for $-\pi < \theta < \pi$.
  }
  \item[(e)]{
    $(-i)^i = e^{i \log (-i)}$, and $-i = e^{-i\frac{\pi}{2}}$ so for
    this branch of the logarithm we have $\log i = -i\frac{\pi}{2}$,
    so $(-i)^i = e^{\frac{\pi}{2}}$. The same value is attained
    for $-\pi < \theta < \pi$.
  }
\end{itemize}

\section{Additional Problems}

\begin{Problem}
  Let $\mathrm{Log} z$ be the principal logarithm function
  defined using $\mathrm{Arg}~z \in (-\pi, \pi]$. Prove that
  $\mathrm{Log}~z$ is holomorphic on
  $\mathbb{C} \backslash \{x \in \mathbb{R} : x \leq 0 \}$ and
  that $\frac{d}{dz} \mathrm{Log}~z = \frac{1}{z}$.
  (Hint: Divide the domain into the union of the right, lower, and
  upper half-planes. Apply the Cauchy-Riemann equations.)
\end{Problem}

\begin{Answer}
  We have $\mathrm{Log}~z = \log |z| + i \mathrm{Arg}~z$.
  Let $z = x + iy = e^{i \theta}$, and write
  $\mathrm{Log}~(x + iy) = u(x, y) + i v(x, y)$.

  \begin{itemize}
    \item{
      In the half-plane $\{ z : \mathrm{Im}~z < 0 \}$ we have
      $\theta \neq 0$, $\theta \neq \pi$, so $\sin \theta \neq 0$
      and thus
      $\cot \theta = \frac{\cos \theta}{\sin \theta} = \frac{x}{y}$ is
      defined. Furthermore $\sin \theta < 0$, and
      with this choice of principal logarithm we have
      $-\pi < \theta < 0$.
      On this domain we then have $\mathrm{Arg}~z = \cot^{-1} \frac{y}{x}$, so
      $$
      \mathrm{Log}~z = \log \sqrt{x^2 + y^2} + i \cot^{-1} \frac{y}{x}
      $$
      so that
      $$
      u(x, y) = \log \sqrt{x^2 + y^2}, \quad
      v(x, y) = \cot^{-1} \frac{x}{y}
      $$
      and then
      \begin{align*}
      u_x &= \left(\frac{\partial}{\partial x} \sqrt{x^2 + y^2}\right)
             \left(\frac{1}{\sqrt{x^2 + y^2}}\right)
           = (2x)\left(\frac{1}{2}(x^2 + y^2)^{-1/2}\right)
             \left(\frac{1}{\sqrt{x^2 + y^2}}\right) \\
          &= \frac{x}{x^2 + y^2}, \\
      u_y &= \frac{y}{x^2 + y^2} \\
      v_x &= \frac{1}{y}\left(-\frac{1}{1 + \left(\frac{x}{y}\right)^2}\right)
           = -\frac{y}{x^2 + y^2} \\
      v_y &= -\frac{x}{y^2}\left(-\frac{1}{1 + \left(\frac{x}{y}\right)^2}\right)
           = \frac{x}{x^2 + y^2},
      \end{align*}
      so the Cauchy-Riemann equations are satisfied.
      We confirm also that
      $$
        u_x + i v_x
      = \frac{x - iy}{x^2 + y^2}
      = \frac{\bar{z}}{|z|}
      = \frac{1}{z},
      $$
      so $\frac{d}{dz} \log z = \frac{1}{z}$ on this domain.
    }
    \item{
      In the half-plane $\{z : \mathrm{Im}~z > 0\}$ we have
      $\theta \neq 0$, $\theta \neq \pi$, so $\sin \theta \neq 0$ and
      $\theta = \cot^{-1} \frac{y}{x}$, so that
      $$
      u(x, y) = \log \sqrt{x^2 + y^2}, \quad
      v(x, y) = \cot^{-1} \frac{x}{y}
      $$
      in this case as well, so the Cauchy-Riemann
      equations are satisfied in this region as well and
      $\frac{d}{dz} \log z = \frac{1}{z}$.
    }
    \item{
      In the half-plane $\{z : \mathrm{Re}~z > 0\}$ we have
      $\theta \neq \pm \frac{\pi}{2}$, so $\cos \theta \neq 0$ and
      $\tan \theta = \frac{\sin \theta}{\cos \theta}$ is defined.
      Therefore $\theta = \tan^{-1} \theta$ so
      $$
      u(x, y) = \log \sqrt{x^2 + y^2}, \quad
      v(x, y) = \tan^{-1} \frac{y}{x}
      $$
      and then
      \begin{align*}
      u_x &= \frac{x}{x^2 + y^2}, \\
      u_y &= \frac{y}{x^2 + y^2} \\
      v_x &= -\frac{y}{x^2}\frac{1}{\frac{y^2}{x^2} + 1}
           = -\frac{y}{x^2 + y^2}, \\
      v_y &= \frac{1}{x}\frac{1}{\frac{y^2}{x^2} + 1}
           = \frac{x}{x^2 + y^2}.
      \end{align*}
      We confirm also that
      $$
      u_x + i v_x = \frac{x - y}{x^2 + y^2} = \frac{1}{z}.
      $$
    }
  \end{itemize}
  Therefore the Cauchy-Riemann equations hold on a union of sets which
  cover the domain of this branch of the logarithm, and the derivative
  is equal to $\frac{1}{z}$ on each set composing this union, so this
  branch of the logarithm is holomorphic on its domain and has
  derivative $\frac{1}{z}$ as desired.
\end{Answer}

\begin{Problem}
  \begin{enumerate}[(i)]
    \item{
      Let $f$, $g$ be two entire functions such that
      $f^\prime(z) = g^\prime(z)$ for all $z$. Show that there is a
      constant $C \in \mathbb{C}$ such that $f = g + C$.
    }
    \item{
      Let $f$ be an entire function and $n \in \mathbb{N}$.
      Suppose $f^{(n)} = 0$. Show that $f$ is a polynomial
      with $\deg f \leq n - 1$.
    }
  \end{enumerate}
\end{Problem}

\begin{Answer}
  \begin{enumerate}[(i)]
    \item{
      Since $f^\prime = g^\prime$, we have $f^\prime - g^\prime = 0$.
      But $f^\prime - g^\prime = (f - g)^\prime$, so since
      $(f - g)^\prime = 0$ this means $f - g = C$ for some constant
      $C$, and then $f = g + C$ as desired.
    }
    \item{
      \begin{itemize}
        \item{
          Consider $n = 1$. Then $f^\prime = 0$, so $f$ is constant,
          i.e. a polynomial of degree $0 = n - 1$.
        }
        \item{
          Suppose $n > 1$ and that the assertion holds for all
          $m < n$, and that $f^{(n)} = \frac{d}{dz} f^{(n-1)} = 0$. Then
          $f^{(n-1)} = C$ for some $C \in \mathbb{C}$,
          so $f^{(n-1)} - C = 0$.

          Define
          $$
          g(z) = f(z) - \frac{C}{(n-1)!} z^{n-1}.
          $$
          Then
          $$
            g^{(n-1)}(z)
          = \frac{d^{n-1}}{dz^{n-1}} \left( f(z) - \frac{C}{(n-1)!}
            z^{n-1} \right)
          = f^{(n-1)}(z) - C
          $$
          and therefore $g^{(n-1)}(z) = 0$. But then by the inductive
          hypothesis $g$ is a polynomial with $\deg g \leq n - 2$, and
          so
          $$
          f(z) = g(z) + \frac{C}{(n-1)!}z^{n-1}
          $$
          is a polynomial with $\deg f = n - 1$.
        }
      \end{itemize}
    }
  \end{enumerate}
\end{Answer}

\begin{Problem}
  Let $f$ be an entire function. Suppose that $|f|$ is constant. Prove
  that $f$ is constant.
  (Hint: $|f| = C$ implies $u^2 + v^2 = C^2$. Take partial derivatives
  and apply the Cauchy-Riemann equations.)
\end{Problem}

\begin{Answer}
  Since $|f| = C$, $|f|^2 = u^2 + v^2 = C^2$. Since $f$ is
  holomorphic, we must have
  \begin{align*}
    0 &= \frac{\partial}{\partial x} (u^2 + v^2)
       = u_x \cdot 2 u + v_x \cdot 2 v \\
      &= 2 u u_x - 2 v u_y
  \end{align*}
  and
  \begin{align*}
    0 &= \frac{\partial}{\partial y} (u^2 + v^2)
       = u_y \cdot 2 u + v_y \cdot 2 v \\
      &= 2 u v_x - 2 v v_y,
  \end{align*}
  so that
  $$
  u u_x = v u_y, \quad
  u v_x = v v_y.
  $$
  Multiplying the first equation by $i$ and adding it to the second we
  have
  \begin{align*}
  u u_x + i u v_x &= v u_y + i v v_y \\
  u (u_x + i v_x) &= v (u_y + i v_y).
  \end{align*}
  But $u_x + i v_x = f^\prime$, and since
  $$
  i f^\prime = i(v_y - i u_y) = u_y + i v_y,
  $$
  we have $u f^\prime = i v f^\prime$ or
  $(u - iv)f^\prime = \bar{f} f^\prime = 0$. Then it must be that
  $\bar{f} = 0 = f$ or $f^\prime = 0$, and in either case this implies that $f$
  is constant.

  If $C = 0$, then $f = 0$. Assume $C > 0$. Differentiating
  $u^2 + v^2 = C^2$ we have $2u u_x + 2 v v_x = 0$ and
  $2 u u_y + 2 v v_y = 0$. The Cauchy-Riemann equations give
  $-2 u v_x + 2 v u_x = 0$. From this we can multiply
  to find
  $$
  v (2u u_x + 2 v v_x) - u(-2 u v_x + 2 v u_x) = 2 (v^2 + u^2) v_x = 2 C^2 v_x = 0
  $$
  and similarly we have $2 (u^2 + v^2) u_x = 2 C^2 u_x = 0$. Since $C > 0$, this
  that $f^\prime = 0$.
\end{Answer}

\begin{Problem}
  Let $f$ be an entire function Suppose that $f^\prime(z) = f(z)$ for
  any $z \in \mathbb{C}$. Prove that $f(z) = C e^z$ for some
  $C \in \mathbb{C}$.
\end{Problem}

\begin{Answer}
Since $f^\prime = u_x + i v_x$, $f^\prime = f$ implies
that $u_x + i v_x = u + i v$, and since $u$ and $v$ are
real functions this in turn implies that $u_x = u$ and
$v_x = v$. Then $u(x, y) = k(y) e^x$ for some function
$k(y)$ that does not depend on $x$, and similarly
$v(x, y) = l(y) e^x$.
We also have $f^\prime = v_y - i u_y$, so
$v_y = u$ and $u_y = -v$. Then
$l^\prime(y) e^x = k(y) e^x$ and
$k^\prime(y) e^x = -l(y) e^x$, so
$l^\prime(y) = k(y)$ and
$k^\prime(y) = -l(y)$. Then
$-l(y) = k^\prime(y) = l^{\prime\prime}(y)$
and $k(y) = l^\prime(y) = -k^{\prime\prime}(y)$, and the unique
solutions to these equations are sinusoids.
Since $l^\prime(y) = k(y)$ this means
$k(y) = K \cos y$ and $l(y) = K \sin y$
for a real constant $K$. We conclude that
$$
  f(x + iy)
= K e^x \cos y + i K e^x \sin y
= K e^{x + iy}
$$
as desired.

Let $g(z) = e^{-z} f(z)$. Then
$g^\prime(z) = e^{-z} f^\prime(z) - e^{-z} f(z) = 0$
since $f^\prime = f$. Therefore $g = C$ so $f(z) = C e^z$.
\end{Answer}

\begin{Problem}
  Let $\sum_{n=0}^\infty a_n z^n$ be a power series with radius $R$.
  \begin{enumerate}[(i)]
    \item{
      If the series diverges at $z = 3 - 4i$, what can you say about $R$?
    }
    \item{
      If the series converges at every $z \in D(0, 1)$, what can you say about
      $R$?
    }
    \item{
      What is the radius of $\sum_{n=0}^\infty a_n z^{2n}$?
    }
  \end{enumerate}
\end{Problem}

\begin{Answer}
  \begin{enumerate}
    \item{
      We must have that the series converges for every $z$ with $|z| <
      R$, so since $|3 - 4i| = \sqrt{3^2 + 4^2} = 5$ it must be that
      $R \leq 5$.
    }
    \item{
      Similarly, since $0 \in D(0,1)$ and $|0| = 0$, we have that
      $R = 0$ since $R \geq 0$ must also be satisfied.
    }
    \item{
      Observe that
      $$
      \sum_{n=0}^\infty a_n z^n + \sum_{n=0}^\infty (-1)^n a_n z^n
      = \sum_{n=0}^\infty 2 a_n z^{2n}
      $$
      so that
      $$
        \sum_{n=0}^\infty a_n z^{2n}
      = \frac{1}{2}\left[
          \sum_{n=0}^\infty (-1)^n a_n z^n
        + \sum_{n=0}^\infty a_n z^n
        \right]
      $$
      Observing that $|(-1)^n a_n|^{\frac{1}{n}} =
      |a_n|^{\frac{1}{n}}$, we see that $\sum (-1)^n a_n z^n$ has the
      same radius of convergence as $\sum a_n z^n$, and the radius of
      convergence of this sum of series is the minimum of the radii of
      convergence of the summands. Therefore this series has the same
      radius of convergence as $\sum a_n z^n$, namely $R$.
    }
  \end{enumerate}
\end{Answer}

\end{document}
